more; tuning decide;

Weidenbach_Book/CDCL_Two_Watched_Literals_Algorithm.thy
@@ -387,22 +387,63 @@ subsection \<open>Other Rules\<close>
 
 subsubsection \<open>Decide\<close>
 
-definition decide :: "'v twl_st \<Rightarrow> 'v twl_st nres" where
-  \<open>decide = (\<lambda>(M, N, U, D, NP, UP, WS, Q). do {
-     L \<leftarrow> SPEC (\<lambda>L. undefined_lit M L \<and> atm_of L \<in> atms_of_mm (clause `# N));
-     RETURN (Decided L # M, N, U, D, NP, UP, WS, {#-L#})
-  })
-\<close>
+definition find_unassigned_lit :: \<open>'v twl_st \<Rightarrow> 'v literal option nres\<close> where
+  \<open>find_unassigned_lit = (\<lambda>S.
+      SPEC (\<lambda>L.
+        (L \<noteq> None \<longrightarrow> undefined_lit (get_trail S) (the L) \<and>
+          atm_of (the L) \<in> atms_of_mm (clause `# get_clauses S)) \<and>
+        (L = None \<longrightarrow> (\<nexists>L. undefined_lit (get_trail S) L \<and>
+         atm_of L \<in> atms_of_mm (clause `# get_clauses S)))))\<close>
 
+definition propagate_dec where
+  \<open>propagate_dec = (\<lambda>L (M, N, U, D, NP, UP, WS, Q). (Decided L # M, N, U, D, NP, UP, WS, {#-L#}))\<close>
+
+definition decide :: "'v twl_st \<Rightarrow> 'v twl_st nres" where
+  \<open>decide S = do {
+     L \<leftarrow> find_unassigned_lit S;
+     case L of
+       None \<Rightarrow> RETURN S
+     | Some L \<Rightarrow> RETURN (propagate_dec L S)
+  }
+\<close>
 
 lemma decide_spec:
   assumes \<open>clauses_to_update S = {#}\<close> and \<open>literals_to_update S = {#}\<close> and \<open>get_conflict S = None\<close> and
     twl: \<open>twl_struct_invs S\<close> and twl_s: \<open>twl_stgy_invs S\<close>
-  shows \<open>decide S \<le> SPEC (\<lambda>T. cdcl_twl_o S T \<and> get_conflict T = None \<and> clauses_to_update T = {#} \<and>
+  shows \<open>decide S \<le> SPEC (\<lambda>T.
+   ((S \<noteq> T \<and> (\<exists>L. undefined_lit (get_trail S) L \<and> atm_of L \<in> atms_of_mm (clause `# get_clauses S)) \<and>
+    cdcl_twl_o S T \<and> literals_to_update T \<noteq> {#}) \<or>
+     (S = T \<and>
+      (\<nexists>L. undefined_lit (get_trail S) L \<and> atm_of L \<in> atms_of_mm (clause `# get_clauses S)) \<and>
+      no_step cdcl_twl_o S )) \<and>
+    get_conflict T = None \<and> clauses_to_update T = {#} \<and>
     twl_struct_invs T \<and> twl_stgy_invs T)\<close>
 proof -
   obtain M N U NP UP where S: \<open>S = (M, N, U, None, NP, UP, {#}, {#})\<close>
     using assms by (cases S) auto
+  have [dest!]:
+    \<open>atm_of L \<in> atms_of_ms (clause ` set_mset N)\<close>
+    if U: \<open>atm_of L \<in> atms_of_ms (clause ` set_mset U)\<close> and
+       undef: \<open>undefined_lit M L\<close>
+    for L
+  proof -
+    have \<open>cdcl\<^sub>W_restart_mset.no_strange_atm (state\<^sub>W_of S)\<close> and unit: \<open>unit_clss_inv S\<close>
+      using twl unfolding twl_struct_invs_def cdcl\<^sub>W_restart_mset.cdcl\<^sub>W_all_struct_inv_def
+      by fast+
+    moreover have \<open>atm_of L \<notin> atms_of_mm NP\<close>
+    proof (rule ccontr)
+      assume \<open>\<not> ?thesis\<close>
+      then obtain C where C: \<open>C \<in># NP\<close> and LC: \<open>atm_of L \<in> atms_of C\<close>
+        by (auto  simp: S atms_of_ms_def atms_of_def)
+      then obtain L' where \<open>C = {#L'#}\<close> and \<open>defined_lit M L'\<close>
+        using unit by (auto simp: S Decided_Propagated_in_iff_in_lits_of_l)
+      then show False
+        using LC undef by (auto simp: atm_of_eq_atm_of)
+    qed
+    ultimately show ?thesis
+      using that
+      by (auto simp: cdcl\<^sub>W_restart_mset.no_strange_atm_def S cdcl\<^sub>W_restart_mset_state image_Un)
+  qed
   {
     fix L
     assume undef: \<open>undefined_lit M L\<close> and L: \<open>atm_of L \<in> atms_of_mm (clause `# N)\<close>
@@ -416,8 +457,9 @@ proof -
     note o twl' twl_s'
   } note H = this
   show ?thesis
-    unfolding S decide_def
-    by (refine_vcg; auto simp: H)
+    using assms unfolding S decide_def find_unassigned_lit_def propagate_dec_def
+    apply (refine_vcg)
+    by (auto simp: H elim!: cdcl_twl_oE simp: cdcl_twl_o.simps)
 qed
 
 declare decide_spec[THEN order_trans, refine_vcg]
@@ -1022,84 +1064,117 @@ declare backtrack_spec[THEN order_trans, refine_vcg]
 
 subsubsection \<open>Full loop\<close>
 
+definition decide_or_skip :: "'v twl_st \<Rightarrow> (bool \<times> 'v twl_st) nres" where
+  \<open>decide_or_skip S =
+     (if (\<exists>L. undefined_lit (get_trail S) L \<and> atm_of L \<in> atms_of_mm (clause `# (get_clauses S)))
+      then do {S \<leftarrow> decide S; RETURN (False, S)}
+      else do {RETURN (True, S)})\<close>
+
+lemma decide_or_skip_spec:
+  assumes \<open>twl_struct_invs S\<close> and \<open>twl_stgy_invs S\<close> and \<open>clauses_to_update S = {#}\<close> and
+    \<open>literals_to_update S = {#}\<close> and \<open>get_conflict S = None\<close> and
+    ns_cp: \<open>no_step cdcl_twl_cp S\<close>
+  shows
+    \<open>decide_or_skip S \<le> SPEC(\<lambda>(brk, T). cdcl_twl_o\<^sup>*\<^sup>* S T \<and>
+       (get_conflict T \<noteq> None \<longrightarrow> get_conflict T = Some {#}) \<and>
+       no_step cdcl_twl_o T \<and> (brk \<longrightarrow> no_step cdcl_twl_stgy T) \<and> twl_struct_invs T \<and>
+       twl_stgy_invs T \<and> clauses_to_update T = {#} \<and>
+       (\<not>brk \<longrightarrow> literals_to_update T \<noteq> {#}) \<and>
+       (\<not>no_step cdcl_twl_o S \<longrightarrow> cdcl_twl_o\<^sup>+\<^sup>+ S T))\<close>
+proof -
+  have [iff]: \<open>\<not> cdcl_twl_cp S T\<close> for T
+    using ns_cp by fast
+
+  show ?thesis
+    unfolding decide_or_skip_def
+    apply (refine_vcg; remove_dummy_vars)
+    \<comment> \<open>initial invariants\<close>
+    subgoal using assms by auto
+    subgoal using assms by auto
+    subgoal using assms by auto
+    subgoal using assms by auto
+    subgoal using assms by auto
+    subgoal using assms by auto
+    subgoal by (auto simp: cdcl_twl_o.simps)
+    subgoal by (auto simp: cdcl_twl_stgy.simps)
+    subgoal by auto
+    subgoal by auto
+    subgoal using assms by auto
+    subgoal using assms by (auto simp: cdcl_twl_o.simps image_Un)
+    subgoal using assms by (auto simp: cdcl_twl_stgy.simps cdcl_twl_o.simps image_Un)
+    subgoal using assms by fast
+    subgoal using assms by fast
+    subgoal using assms by fast
+    subgoal using assms by fast
+    subgoal using assms by (auto simp: cdcl_twl_o.simps image_Un)
+    done
+qed
+
+declare decide_or_skip_spec[THEN order_trans, refine_vcg]
+
 definition cdcl_twl_o_prog :: "'v twl_st \<Rightarrow> (bool \<times> 'v twl_st) nres" where
   \<open>cdcl_twl_o_prog S =
     do {
-      let (M, N, U, D, NP, UP, WS, Q) = S in
-      do {
-        if D = None
-        then
-          if (\<exists>L. undefined_lit M L \<and> atm_of L \<in> atms_of_mm (clause `# N))
-          then do {S \<leftarrow> decide S; RETURN (False, S)}
-          else do {RETURN (True, S)}
-        else do {
-          T \<leftarrow> skip_and_resolve_loop S;
-          if get_conflict T \<noteq> Some {#}
-          then do {U \<leftarrow> backtrack T; RETURN (False, U)}
-          else do {RETURN (True, T)}
-        }
+      if get_conflict S = None
+      then decide_or_skip S
+      else do {
+        T \<leftarrow> skip_and_resolve_loop S;
+        if get_conflict T \<noteq> Some {#}
+        then do {U \<leftarrow> backtrack T; RETURN (False, U)}
+        else do {RETURN (True, T)}
       }
     }
   \<close>
 
-
 lemma cdcl_twl_o_prog_spec:
-  assumes \<open>twl_struct_invs S\<close> and \<open>twl_stgy_invs S\<close> and \<open>clauses_to_update S = {#}\<close> and \<open>literals_to_update S = {#}\<close> and
+  assumes \<open>twl_struct_invs S\<close> and \<open>twl_stgy_invs S\<close> and \<open>clauses_to_update S = {#}\<close> and
+    \<open>literals_to_update S = {#}\<close> and
     ns_cp: \<open>no_step cdcl_twl_cp S\<close>
   shows
-    \<open>cdcl_twl_o_prog S \<le> SPEC(\<lambda>(brk, T). cdcl_twl_o\<^sup>*\<^sup>* S T \<and> (get_conflict T \<noteq> None \<longrightarrow> get_conflict T = Some {#}) \<and>
-      no_step cdcl_twl_o T \<and> (brk \<longrightarrow> no_step cdcl_twl_stgy T) \<and> twl_struct_invs T \<and>
-      twl_stgy_invs T \<and> clauses_to_update T = {#} \<and>
-      (\<not>brk \<longrightarrow> literals_to_update T \<noteq> {#}) \<and>
-      (\<not>no_step cdcl_twl_o S \<longrightarrow> cdcl_twl_o\<^sup>+\<^sup>+ S T))\<close>
+    \<open>cdcl_twl_o_prog S \<le> SPEC(\<lambda>(brk, T). cdcl_twl_o\<^sup>*\<^sup>* S T \<and>
+       (get_conflict T \<noteq> None \<longrightarrow> get_conflict T = Some {#}) \<and>
+       no_step cdcl_twl_o T \<and> (brk \<longrightarrow> no_step cdcl_twl_stgy T) \<and> twl_struct_invs T \<and>
+       twl_stgy_invs T \<and> clauses_to_update T = {#} \<and>
+       (\<not>brk \<longrightarrow> literals_to_update T \<noteq> {#}) \<and>
+       (\<not>no_step cdcl_twl_o S \<longrightarrow> cdcl_twl_o\<^sup>+\<^sup>+ S T))\<close>
     (is \<open>_ \<le> ?S\<close>)
-  unfolding cdcl_twl_o_prog_def
-  apply (refine_vcg; remove_dummy_vars)
-  \<comment> \<open>initial invariants\<close>
-  subgoal using assms by auto
-  subgoal using assms by auto
-  subgoal using assms by auto
-  subgoal using assms by auto
-  subgoal using assms by auto
-  \<comment> \<open>decision, if false\<close>
-  subgoal using assms by (auto elim!: cdcl_twl_oE)
-  subgoal using assms by auto
-  subgoal using assms by (auto elim!: cdcl_twl_oE)
-  subgoal using assms by auto
-  subgoal using assms by (auto elim!: cdcl_twl_oE)
-  subgoal for M N D NP UP WS Q brk T
-    by (cases T) (use ns_cp in \<open>auto elim!: cdcl_twl_stgyE cdcl_twl_oE\<close>)
-  subgoal using assms by auto
-  subgoal using assms by auto
-  subgoal using assms by auto
-  subgoal using assms by auto
-  subgoal by (auto elim!: cdcl_twl_oE)
+proof -
+  have [iff]: \<open>\<not> cdcl_twl_cp S T\<close> for T
+    using ns_cp by fast
 
-  \<comment> \<open>\<^term>\<open>skip_and_resolve_loop\<close> part, if true\<close>
-    \<comment> \<open>initial conditions\<close>
-  subgoal using assms by auto
-  subgoal using assms by auto
-  subgoal using assms by (auto elim!: cdcl_twl_oE)
-  subgoal using assms by auto
+  show ?thesis
+    unfolding cdcl_twl_o_prog_def
+    apply (refine_vcg decide_spec[THEN order_trans]; remove_dummy_vars)
+    \<comment> \<open>initial invariants\<close>
+    subgoal using assms by auto
+    subgoal using assms by auto
+    subgoal using assms by auto
+    subgoal using assms by auto
+    subgoal using assms by auto
+    subgoal using assms by auto
+    subgoal using assms by auto
+    subgoal using assms by auto
+    subgoal using assms by auto
+    subgoal using assms by auto
+    subgoal using assms by auto
+    subgoal using assms by auto
+    subgoal for x T using assms
+      by (cases T) (auto elim!: cdcl_twl_stgyE cdcl_twl_oE)
 
-    \<comment> \<open>initial of backtrack part\<close>
-  subgoal by auto
-  subgoal by auto
-  subgoal by auto
+    \<comment> \<open>decision, if false\<close>
+    subgoal using assms by (auto elim!: cdcl_twl_oE)
+    subgoal using assms by (auto elim!: cdcl_twl_oE)
+    subgoal using assms by (auto simp: cdcl_twl_o.simps image_Un)
 
-    \<comment> \<open>final properties\<close>
-  subgoal by (auto elim!: cdcl_twl_oE)
-  subgoal by auto
-  subgoal by auto
-  subgoal by blast
-  subgoal by fast
-  subgoal by (auto elim!: cdcl_twl_oE)
-  subgoal by (auto elim!: cdcl_twl_stgyE cdcl_twl_oE cdcl_twl_cpE)
-  subgoal by fast
-  subgoal by (auto simp: rtranclp_unfold elim!: cdcl_twl_oE)
-  done
+    subgoal using assms ns_cp by (auto simp: cdcl_twl_o.simps  cdcl_twl_stgy.simps image_Un)
+    subgoal using assms by (auto elim!: cdcl_twl_oE simp: cdcl_twl_o.simps  cdcl_twl_stgy.simps image_Un cdcl_twl_cp.simps)
+    subgoal using assms by auto
+    subgoal by (auto simp: rtranclp_unfold elim!: cdcl_twl_oE)
+    done
+qed
 
 declare cdcl_twl_o_prog_spec[THEN order_trans, refine_vcg]
+
 
 subsection \<open>Full Strategy\<close>
 
